List take/drop

opentheory/stdlib/all.ml
@@ -2,6 +2,7 @@
 (* Additions to the OpenTheory standard library.                             *)
 (* ------------------------------------------------------------------------- *)
 
+loads "opentheory/stdlib/tactics.ml";;
 loads "opentheory/stdlib/option.ml";;
 loads "opentheory/stdlib/list.ml";;
 
