opentheory/stdlib/tactics.ml
@@ -1,0 +1,17 @@
+(* ------------------------------------------------------------------------- *)
+(* Additional tactics to support the OpenTheory standard library             *)
+(* ------------------------------------------------------------------------- *)
+
+(* Pretty useless without also making THEN1 infix... *)
+let (THEN1) = fun tac1 tac2 -> tac1 THENL [tac2; ALL_TAC];;
+
+let PAT_ASSUM pat =
+    let is_pat th = can (term_match [] pat) (concl th) in
+    FIRST_X_ASSUM (fun th -> if is_pat th then MP_TAC th else NO_TAC);;
+
+let KNOW_TAC =
+    let th = ITAUT `!x y. x /\ (x ==> y) ==> y` in
+    fun tm ->
+      MATCH_MP_TAC th THEN
+      EXISTS_TAC tm THEN
+      CONJ_TAC;;
